<?xml version="1.0" encoding="UTF-8"?>

<pretext>
  <article xml:id="article">
    <worksheet margin="1in" bottom="1.25in" xml:id="ws-trigsub">
      <title>Worksheet for Section 6.2: Trigonometric Substitution</title>

      <objectives>
        <ul>
          <li>
            <p>
              Evaluate integrals using trigonometric substitution.
            </p>
          </li>
        </ul>
      </objectives>

      <introduction>
        <p>
          Evaluate the integrals.
          In the case of a definite integral, your answer should be a number.
          For indefinite integrals, your answer should be the most general antiderivative (this means don&#2019;t forget <m>+C</m>).
        </p>
      </introduction>


      <page>
        <exercise>
          <statement>
            <p>
              <m>\int_0^2\sqrt{4-x^2}\,dx</m>
            </p>
          </statement>

          <solution>
            <p>
              Let <m>x = 2 \sin \theta</m>, so that <m>dx = 2 \cos \theta\,d\theta</m> and <m>\sqrt{4-x^2} = 2 \cos\theta</m>.
              Also, <m>\theta =0</m> when <m>x=0</m> and <m>\theta=\pi/2</m> when <m>x=2</m>.
              So
              <me>
                \begin{aligned} \int_0^2\sqrt{4-x^2}\,dx &amp;= 4\int_0^{\pi/2} \cos^2 (\theta)\,d\theta \\ &amp;= 4\int_0^{\pi/2} \frac{1+\cos(2\theta)}{2}\,d\theta \\ &amp;= 2\int_0^{\pi/2} \left(1+\cos(2\theta)\right)\,d\theta \\ \end{aligned}
              </me>
              Now <m>\int_0^{\pi/2} 1 \,d\theta</m> is clearly <m>\frac{\pi}{2}</m>.
              What about <m>\int_0^{\pi/2} \cos(2\theta)\,d\theta</m>? There is a way to make it go away.
              Notice that the sinusoidal functions spend as much time above the axis as below the axis.
              The integral of cosine from <m>0</m> to <m>\pi</m> is <m>0</m>.
              But <m>\cos(2\theta)</m> has twice the frequency, so half the period, so the integral is zero again.
            </p>

            <p>
              Putting this together, we have
              <me>
                \int_0^2\sqrt{4-x^2}\,dx = \pi
              </me>
              Notice this integral measures the area of a quarter of the circle of radiusÂ 2.
              So this jives with our well-known formula for the area of a circle.
            </p>
          </solution>
        </exercise>

        <exercise>
          <statement>
            <p>
              <m>\int\frac{dx}{\sqrt{x^2 + 3}}</m>
            </p>
          </statement>

          <solution>
            <p>
              Let <m>x = \sqrt{3} \tan\theta</m>, so <m>dx = \sqrt{3}\sec^2\theta\,d\theta</m> and <m>\sqrt{x^2 + 3} = \sqrt{3}\sec\theta</m>.
              Then
              <me>
                \begin{aligned} \int\frac{dx}{\sqrt{x^2 + 3}} &amp;= \int\frac{\sqrt{3}\sec^2\theta}{\sqrt{3}\sec\theta}\,d\theta \\ &amp;= \int \sec\theta \,d\theta \\ &amp;= \ln| \sec\theta + \tan\theta| + C \\ \end{aligned}
              </me>
            </p>

            <p>
              If <m>x=\sqrt{3} \tan\theta</m>, then <m>\tan\theta=\frac{x}{\sqrt{3}}</m>, which means <m>\sec\theta=\frac{\sqrt{x^2+3}}{\sqrt{3}}</m>.
            </p>

            <image width="60%">
              <prefigure xmlns="https://prefigure.org" label="secant-tangent-diagram">
              <diagram dimensions="(300,300)" margins="10">
              <coordinates bbox="(-1,-1,2,2)">
              <definition>
p1 = [0,0]
              </definition>

              <definition>
p2 = [sqrt(3),0]
              </definition>

              <definition>
p3 = [sqrt(3),2]
              </definition>

              <definition>
v = p3 - p1
              </definition>

              <definition>
th = degrees(atan2(v[1],v[0]))
              </definition>
              <triangle vertices="(p1,p2,p3)" />
              <label anchor="0.5*(p1+p2)" alignment="s"><m>\sqrt{3}</m></label>
              <label anchor="0.5*(p2+p3)" alignment="e"><m>x</m></label>
              <!-- I wanted rotate="th" here but it didn't work -->
              <label anchor="0.5*(p1+p3)" alignment="n"
                      rotate="49.107" 
                    ><m>\sqrt{x^2+3}</m></label>
              <angle-marker points="(p2,p1,p3)"><m>\theta</m></angle-marker>
              </coordinates>
              </diagram>
              </prefigure>
            </image>

            <p>
              So
              <me>
                \begin{aligned} \int\frac{dx}{\sqrt{x^2 + 3}} &amp;= \ln\left| \frac{\sqrt{x^2+3}}{3} + \frac{x}{\sqrt{3}}\right| + C \\ &amp;= \ln\left| \frac{\sqrt{x^2+3}+x}{3}\right| + C \\ &amp;= \ln\left| \sqrt{x^2+3}+x\right| - \ln\sqrt{3} + C \\ &amp;= \ln\left| \sqrt{x^2+3}+x\right| + C \\ \end{aligned}
              </me>
              The constants on the last two lines are different!
            </p>
          </solution>
        </exercise>

        <exercise>
          <statement>
            <p>
              <m>\int \sqrt{x^2-9}\,dx</m>.
            </p>
          </statement>

          <solution>
            <p>
              Let <m>x=3 \sec\theta</m>, so <m>dx = 3 \sec\theta\tan\theta\,d\theta</m> and <m>\sqrt{x^2-9} = 3 \tan\theta</m>.
              Then
              <me>
                \begin{aligned} \int \sqrt{x^2-9}\,dx &amp;= 9 \int\tan^2\theta\sec\theta\,d\theta \\ &amp;= 9 \int(\sec^2\theta-1)\sec\theta\,d\theta \\ &amp;= 9 \left\{\int\sec^3 \theta\,d\theta - \int\sec\theta \,d\theta\right\} \\ &amp;= 9 \left\{\frac{1}{2}\left(\sec\theta\tan\theta+\ln|\sec\theta + \tan \theta|\right) - \ln|\sec\theta + \tan\theta|\right\} + C\\ &amp;= \frac{9}{2} \sec\theta\tan\theta - \frac{9}{2}\ln|\sec\theta + \tan \theta| + C \\ \end{aligned}
              </me>
              If <m>x=3 \sec\theta</m>, then <m>\sec\theta=\frac{x}{3}</m>:
            </p>

            <p>
              We see <m>\tan\theta=\frac{\sqrt{x^2-9}}{3}</m>.
              <me>
                \begin{aligned} \int \sqrt{x^2-9}\,dx &amp;= \frac{9}{2}\cdot \frac{x}{3} \cdot\frac{\sqrt{x^2-9}}{3} - \frac{9}{2} \ln\left|\frac{x}{3} + \frac{\sqrt{x^2-9}}{3}\right| + C \\ &amp;= \frac{1}{2} x \sqrt{x^2-9} - \frac{9}{2}\ln|x + \sqrt{x^2-9}| + C \end{aligned}
              </me>
              The <m>C</m> on the last line is different from the one on the penultimate line; as in the last problem we have subsumed the <m>-\ln 3</m> constant.
              See <url href="http://wolfr.am/150uZMy">http://wolfr.am/150uZMy</url>.
            </p>
          </solution>
        </exercise>
      </page>


      <page>
        <exercise>
          <statement>
            <p>
              <m>\int x^2\sqrt{4-3x^2}\,dx</m>
            </p>
          </statement>

          <solution>
            <p>
              This time let <m>\sqrt{3} x = 2 \sin\theta</m>.
              Then <m>\sqrt{3} \,dx = 2 \cos\theta\,d\theta</m> and <m>\sqrt{4-3x^2} = 2 \cos \theta</m>.
              So
              <me>
                \begin{aligned} \int x^2\sqrt{4-3x^2}\,dx &amp;= \int\frac{4}{3} \sin^2\theta \cdot 2 \cos \theta \cdot \frac{2}{\sqrt 3} \cos\theta\,d\theta \\ &amp;= \frac{16}{3\sqrt{3}} \int\sin^2\theta \cos^2\theta\,d\theta \\ &amp;= \frac{4}{3\sqrt{3}} \int \sin^2(2\theta)\,d\theta\\ &amp;= \frac{2}{3\sqrt{3}} \int (1-\cos(4\theta))\,d\theta \\ &amp;= \frac{2}{3\sqrt{3}}\theta - \frac{1}{6\sqrt{3}}\sin(4\theta) + C \end{aligned}
              </me>
              To put this back in terms of <m>x</m>, use the identity
              <me>
                \sin(4\theta) = 2 \sin(2\theta)\cos(2\theta) = 4 \sin(\theta)\cos(\theta)(1-2\sin^2\theta)
              </me>
              then unsubstitute <m>\theta = \arcsin\left(\frac{\sqrt{3}}2 x\right)</m>, <m>\sin\theta = \frac{\sqrt{3}x}{2}</m>, and <m>\cos\theta=\frac{\sqrt{4-3x^2}}{2}</m>.
              So
              <me>
                \begin{aligned} \int x^2\sqrt{4-3x^2}\,dx &amp;= \frac{2}{3\sqrt{3}} \arcsin\left(\frac{\sqrt{3}}{2}x\right) - \frac{1}{6\sqrt{3}}\cdot 4 \cdot \frac{\sqrt{3}}{2}x \cdot \frac{\sqrt{4-3x^2}}{2} \cdot \left(1 - \frac{3}{2}x^2\right) + C \\ &amp;= \frac{2}{3\sqrt{3}} \arcsin\left(\frac{\sqrt{3}}{2}x\right) - \frac{1}{6} x \sqrt{4-3x^2}\left(1 - \frac{3}{2}x^2\right) + C \\ &amp;= \frac{2}{3\sqrt{3}} \arcsin\left(\frac{\sqrt{3}}{2}x\right) + \frac{1}{12} x \sqrt{4-3x^2}\left(3x^2-2\right) + C \\ \end{aligned}
              </me>
            </p>
          </solution>
        </exercise>

        <exercise>
          <statement>
            <p>
              <m>\int_{\ln(3/4)}^{\ln(4/3)} \frac{e^{t}}{(1+e^{2t})^{3/2}}\,dt</m>
            </p>
          </statement>

          <solution>
            <p>
              Let <m>u = e^t</m>.
              Then <m>du = e^t \,dt</m> and
              <me>
                \int_{\ln(3/4)}^{\ln(4/3)} \frac{e^t\,dt}{(1+e^{2t})^{3/2}} = \int_{3/4}^{4/3}\frac{du}{(1+u^2)^{3/2}}.
              </me>
              Now let <m>u = \tan\theta</m>.
              Then <m>du = \sec^2\theta\,d\theta</m> and
              <me>
                \begin{split} \int_{3/4}^{4/3}\frac{du}{(1+u^2)^{3/2}} &amp;= \int_{\arctan(3/4)}^{\arctan(4/3)} \frac{\sec^2\theta\,d\theta}{\sec^3\theta} \\ &amp;= \int_{\arctan(3/4)}^{\arctan(4/3)} \cos\theta\,d\theta \\ &amp;= \left.\sin\theta\right|_{\arctan(3/4)}^{\arctan(4/3)} \\ &amp;= \frac{4}{5} - \frac{3}{5} = \frac{1}{5}.
                \end{split}
              </me>
            </p>
          </solution>
        </exercise>
      </page>
    </worksheet>
  </article>
</pretext>