<?xml version="1.0" encoding="UTF-8"?>

<pretext>
  <article xml:id="article">
    <!-- When creating a new activity, make a copy of this file with appropriate name -->
    <worksheet margin="1in" bottom="1.25in" xml:id="ws-ibp">
      <title>Worksheet for Section 6.1</title>

      <objectives>
        <ul>
          <li>
            <p>
              Use integration by parts to find the antiderivative of a product of functions.
            </p>
          </li>

          <li>
            <p>
              Use integration by parts to evaluate definite integrals.
            </p>
          </li>
        </ul>
      </objectives>


      <page>
        <exercisegroup>
        <title>The basics</title>

        <introduction>
          <p>
            Evaluate the integrals, integrating by parts.
            In the case of a definite integral, your answer should be a number.
            For indefinite integrals, your answer should be the most general antiderivative (this means don’t forget <m>+C</m>).
          </p>

          <p>
            Think about your choices of <m>u</m> and <m>dv</m>.
            Why did you decide the way you did?
          </p>
        </introduction>

        <exercise workspace="1in">
          <statement>
            <p>
              <m>\int x\sin 2x \,dx</m>
            </p>
          </statement>

          <solution>
            <p>
              Let <m>u = x</m>, so <m>dv = \sin 2x\,dx</m>.
              It follows that <m>du = dx</m> and <m>v = -\frac12\cos 2x</m>.
              So
              <me>
                \begin{aligned} \int x\sin 2x \,dx &amp;= x \cdot \left(-\frac12\cos 2x\right) - \int \left(-\frac12\cos 2x\right) \,dx \\ &amp;= -\frac12 x \cos 2x + \frac12 \cos 2x\,dx \\ &amp;= -\frac12 x \cos 2x + \frac14 \sin 2x + C \end{aligned}
              </me>
            </p>
          </solution>
        </exercise>

        <exercise workspace="1in">
          <statement>
            <p>
              <m>\int t^2 \cos t\,dt</m>
            </p>
          </statement>

          <solution>
            <p>
              First, let <m>u=t^2</m>, <m>dv = \cos t\,dt</m>.
              Then <m>du = 2t \,dt</m> and <m>v = \sin t</m>.
              So
              <me>
                \int t^2 \cos t\,dt = t^2 \sin t - 2\int t \sin t\,dt
              </me>
              We’re not done, but this is better.
              We can integrate by parts again with <m>u = t</m>, <m>du = \sin t\,dt</m>.
              Then <m>du = dt</m> and <m>v = -\cos t</m>.
              So
              <me>
                \int t \sin t \,dt = -t\cos t + \int \cos t\,dt = -t\cos t + \sin t.
              </me>
              Therefore
              <me>
                \begin{split} \int t^2 \cos t\,dt &amp;= t^2 \sin t - 2\left\{-t\cos t + \sin t\right\} \\ &amp;= t^2 \sin t + 2t \cos t - 2 \sin t + C \end{split}
              </me>
            </p>
          </solution>
        </exercise>

        <exercise workspace="1in">
          <statement>
            <p>
              <m>\int_1^2 x \ln x\,dx</m>
            </p>
          </statement>

          <solution>
            <p>
              Let <m>u = \ln x</m>, <m>dv = x\,dx</m>.
              then <m>du = \frac{1}{x}\,dx</m> and <m>v = \frac12x^2</m>.
              <me>
                \begin{split} \int_1^2 x \ln x\,dx &amp;= \left.\frac12 x^2 \ln x\right|^2_1 - \frac12\int_1^2 x\,dx \\ &amp;= \left(\frac12 \cdot 2^2 \cdot \ln 2 - \frac12\cdot 1^2 \cdot \ln 1\right) - \left.\frac14x^2\right|_1^2 \\ &amp;= 2 \ln 2 - \left(1 - \frac14\right) = 2 \ln 2 - \frac34 \end{split}
              </me>
            </p>

            <p>
              Suppose we had tried the other way? You may or may not know that
              <me>
                \int \ln x \,dx = x \ln x - x
              </me>
              (this can be verified directly, or derived by integration by parts).
              So one could do <m>u = x</m>, <m>dv = \ln x\,dx</m>, with <m>du = dx</m>, <m>v = x \ln x - x</m>.
              So
              <me>
                \begin{split} \int_1^2 x \ln x\,dx &amp;= \left[x^2 \ln x - x^2\right]^2_1 - \int_1^2\left(x \ln x - x\right) \,dx \\ &amp;= \left[(4 \ln 2 - 4) - (1 \ln 1 - 1)\right] + \int_1^2 x\,dx - \int_1^2 x\ln x\,dx.
                \end{split}
              </me>
              It appears we’re right back where we’ve started, but actually, we can go forward by adding the last integral to the left-hand side.
              We get
              <me>
                \begin{aligned} 2\int_1^2 x \ln x\,dx &amp;= 4 \ln 2 - 3 + \int_1^2 x\,dx = 4 \ln 2 - 3 + \left.\frac12 x^2 \right|_1^2 \\ \implies \int_1^2 x \ln x\,dx &amp;= 2 \ln 2 - \frac32 + \frac14\left(4-1\right) = 2 \ln 2 - \frac34 \end{aligned}
              </me>
            </p>
          </solution>
        </exercise>
        </exercisegroup>
      </page>


      <page>
        <exercise workspace="1in">
          <title>Dirty Tricks, part I</title>

          <introduction>
            <p>
              We will use integration by parts twice to find <m>\int e^{-2x}\sin 3x\,dx</m>.
            </p>
          </introduction>


          <task>
            <statement>
              <p>
                First use <m>u = \sin 3x</m>, <m>dv = e^{-2x}\,dx</m>.
                The result should contain another integral suitable for integration by parts.
              </p>
            </statement>

            <solution>
              <p>
                Let <m>u=\sin(3x)</m>, <m>dv = e^{-2x}\,dx</m>.
                Then <m>du = 3\cos(3x)\,dx</m> and <m>v = -\frac12e^{-2x}</m>.
                So
                <me>
                  \begin{aligned} I &amp;= -\frac{1}{2}e^{-2x}\sin(3x) + \frac32 \int e^{-2x} \cos(3x)\,dx \\ \end{aligned}
                </me>
              </p>
            </solution>
          </task>


          <task>
            <statement>
              <p>
                Find the remaining integral by parts using <m>dv = \cos 3x\,dx</m> (or some constant multiple of <m>\cos 3x</m>).
                What happens?
              </p>
            </statement>

            <solution>
              <p>
                If <m>dv = \cos 3x\,dx</m>, then <m>u = e^{-2x}</m>.
                So <m>v = \frac13 \sin 3x</m> and <m>du = -2 e^{-2x}\,dx</m>.
                Thus
                <me>
                  \int e^{-2x} \cos(3x)\,dx = \frac13 e^{-2x}\sin 3x + \frac23 \int e^{-2x}\sin 3x\,dx
                </me>
                Putting this together with the first part gives
                <me>
                  \begin{split} \int e^{-2x}\sin 3x\,dx &amp;= -\frac{1}{2}e^{-2x}\sin(3x) + \frac32 \int e^{-2x} \cos(3x)\,dx \\ &amp;= -\frac{1}{2}e^{-2x}\sin(3x) + \frac32 \left\{\frac13 e^{-2x}\sin 3x + \frac23 \int e^{-2x}\sin 3x\,dx\right\} \\ &amp;= \int e^{-2x}\sin 3x\,dx \end{split}
                </me>
                We have come exactly full circle, and the reason why is that our second integration by parts undid the first one.
              </p>
            </solution>
          </task>


          <task>
            <statement>
              <p>
                Try the same thing now with <m>u = \cos 3x</m>.
                What happens now?
              </p>
            </statement>

            <solution>
              <p>
                This time,
                <me>
                  \int e^{-2x}\sin 3x\,dx = -\frac12 e^{-2x} \cos (3x) -\frac32 \int e^{-2x} \sin(3x)\,dx
                </me>
                so
                <me>
                  \begin{aligned} \int e^{-2x}\sin 3x\,dx &amp;= -\frac{1}{2}e^{-2x}\sin(3x) + \frac32\left\{ -\frac12 e^{-2x} \cos (3x) -\frac32 \int e^{-2x} \sin(3x)\,dx \right\} \\ &amp;= -\frac{1}{2}e^{-2x}\sin(3x) - \frac34 e^{-2x} \cos(3x) -\frac{9}{4} \int e^{-2x}\sin 3x\,dx \\ \end{aligned}
                </me>
                We are back where we started, but in a good way.
                <me>
                  \begin{aligned} \frac{13}{4} \int e^{-2x}\sin 3x\,dx &amp;= -\frac{1}{2}e^{-2x}\sin(3x) - \frac34 e^{-2x} \cos(3x) +C\\ \implies \int e^{-2x}\sin 3x\,dx &amp;= -\frac{2}{13}e^{-2x}\sin(3x) - \frac{3}{13} e^{-2x} \cos(3x)+C \end{aligned}
                </me>
              </p>
            </solution>
          </task>
        </exercise>
      </page>


      <page>
        <exercisegroup>
        <title>Combining Techniques</title>

        <introduction>
          <p>
            Try a substitution which transforms the integral into one suitable for parts.
          </p>
        </introduction>

        <exercise workspace="1in">
          <statement>
            <p>
              <m>\int e^{\sqrt{3x+9}}\,dx</m>
            </p>
          </statement>

          <solution>
            <p>
              Let’s try <m>y = \sqrt{3x+9}</m>.
              Then <m>dy = 3\,dx</m> and <m>dx = \frac{1}{3}</m>.
              So
              <me>
                \int e^{\sqrt{3x+9}}\,dx = \frac{1}{3} \int e^{\sqrt{y}}\,dy
              </me>
              Let’s factor this creatively.
              We can’t antidifferentiate <m>e^{\sqrt{y}}</m> simply, but we could do <m>\frac{e^{\sqrt{y}}}{2\sqrt{y}}</m>.
              So let <m>dv = \frac{e^{\sqrt{y}}}{2 \sqrt{y}}\,dy</m>, so that <m>u = 2 \sqrt{y}</m>.
              Therefore <m>v = e^{\sqrt{y}}</m>, <m>du = \frac{1}{2\sqrt{y}} \,dy</m>, and
              <me>
                \frac{1}{3} \int e^{\sqrt{y}}\,dy = \frac{2}{3} \left\{ \sqrt{y} e^{\sqrt{y}} - \int e^{\sqrt{y}} \frac{1}{2\sqrt{y}}\,dy \right\}
              </me>
              For the remaining integral let <m>s = \sqrt{y}</m>, so <m>ds = \frac{1}{2\sqrt{y}}\,dy</m>.
              We have
              <me>
                \begin{split} \frac{1}{3} \int e^{\sqrt{y}}\,dy &amp;= \frac{2}{3} \left\{ \sqrt{y} e^{\sqrt{y}} - e^s + C\right\} \\ &amp;= \frac{2}{3} \sqrt{3x+9} e^{\sqrt{3x+9}} - \frac{2}{3} e^{\sqrt{3x+9}} + C \end{split}
              </me>
            </p>

            <p>
              Here is another attempt: try the substitution <m>y = \sqrt{3x+9}</m>, for the simple reason that it would be nice if that went way.
              Then <m>y^2 = 3x + 9</m>, so <m>2y\,dy = 3\,dx</m>, and thus
              <me>
                \int e^{\sqrt{3x+9}}\,dx = \frac23 \int ye^y\,dy
              </me>
              We then integrate this by parts with <m>u = y</m>, <m>dv = e^y\,dy</m> to get
              <me>
                \int e^{\sqrt{3x+9}}\,dx = \frac23 \left\{y e^y - e^y\right\} + C = \frac23 \sqrt{3x+9}e^{\sqrt{3x+9}} - \frac23 e^{\sqrt{3x+9}} + C
              </me>
            </p>
          </solution>
        </exercise>

        <exercise workspace="1in">
          <statement>
            <p>
              <m>\int\sin(\ln x)\,dx</m>
            </p>
          </statement>

          <solution>
            <p>
              Let <m>y = \ln x</m>, so that <m>x = e^y</m> and <m>dx = e^y\,dy</m>.
              So
              <me>
                \int\sin(\ln x)\,dx = \int e^y \sin y \,dy
              </me>
              So we can do the old integrate-by-parts-twice trick as in #5 to get
              <me>
                \begin{split} \int e^y \sin y \,dy &amp;= \frac12 e^y \sin y - \frac12 e^y \cos y + C \\ &amp;=\frac12 x \sin (\ln x) - \frac12 x \cos(\ln x) + C \end{split}
              </me>
              And if you don’t believe that, try and differentiate.
            </p>
          </solution>
        </exercise>

        <exercise workspace="1in">
          <statement>
            <p>
              Use a trigonometric identity, then integrate by parts: <m>\int_0^{\pi/3} x\tan^2 x\,dx</m>
            </p>
          </statement>

          <solution>
            <p>
              The identity is
              <me>
                1 + \tan^2x = \sec^2 x
              </me>
              This comes from taking <m>\cos^2 + \sin^2 x = 1</m> and dividing both sides by <m>\cos^2 x</m>.
              So
              <me>
                \int_0^{\pi/3} x\tan^2 x\,dx = \int_0^{\pi/3} x\left(\sec^2 x - 1\right)\,dx = \int_0^{\pi/3} x \sec^2 x\,dx - \int_0^{\pi/3} x\,dx
              </me>
              The second integral on the right-hand side is easy, the other one we can do with integration by parts.
              Let <m>dv = \sec^2 x\,dx</m>, so that <m>u = x</m>, <m>du = dx</m>, and <m>v = \tan x</m>.
              Thus
              <me>
                \begin{split} \int_0^{\pi/3} x\tan^2 x\,dx &amp;= \left.x \tan x \right|^{\pi/3}_0 - \int^{\pi/3}_0 \tan x \,dx -\left.\frac12x^2\right|^{\pi/3}_0 \\ &amp;=  \left[x \tan x - \ln \abs{\sec x} - \frac12 x^2\right]^{\pi/3}_0 \\ &amp;=  \frac{\pi}{3} \tan \left(\frac{\pi}{3}\right) - \ln \abs{\sec\left(\frac{\pi}{3}\right)} - \frac{1}{2}\left(\frac{\pi}{3}\right)^2 \\ &amp;= \frac{\pi}{3}\cdot \sqrt{3} - \ln 2 - \frac{\pi^2}{18} \end{split}
              </me>
              Yikes!
            </p>
          </solution>
        </exercise>
        </exercisegroup>
      </page>


      <page>
        <exercisegroup>
        <title>Dirty tricks, part II</title>

        <introduction>
          <p>
            Use integration by parts with <m>dv = dx</m> to find the antiderivatives.
          </p>
        </introduction>

        <exercise workspace="1in">
          <statement>
            <p>
              <m>\int\arctan x\,dx</m>
            </p>
          </statement>

          <solution>
            <p>
              Let <m>u = \arctan x</m>, <m>dv = dx</m>.
              Then <m>du = \frac{dx}{1+x^2}</m>, and <m>v = x</m>.
              So
              <me>
                \int\arctan x\,dx = x \arctan x - \int \frac{x}{1+x^2}\,dx
              </me>
              The last integral can be done by substituting <m>y = 1 + x^2</m>, <m>dy = 2x\,dx</m>.
              So
              <me>
                \int\arctan x\,dx = x \arctan x - \frac12 \ln(1+x^2) + C
              </me>
            </p>
          </solution>
        </exercise>

        <exercise workspace="1in">
          <statement>
            <p>
              <m>\int\operatorname{arcsec} x\,dx</m>
            </p>
          </statement>

          <solution>
            <p>
              Let <m>u=\operatorname{arcsec}x</m>, <m>du = \frac{1}{x\sqrt{x^2-1}}\,dx</m>.
              So <m>dv = dx</m>, <m>v = x</m>.
              Thus
              <me>
                \int\operatorname{arcsec} x\,dx = x \operatorname{arcsec}x - \int \frac{dx}{\sqrt{x^2-1}}
              </me>
              Oops…we don’t actually know how to do that last integral.
              But here’s the rabbit out the hat:
              <me>
                \int\operatorname{arcsec} x\,dx = x \operatorname{arcsec}x - \ln\abs{x + \sqrt{x^2-1}} + C
              </me>
            </p>
          </solution>
        </exercise>
        </exercisegroup>
      </page>


      <page>
        <exercise workspace="1in">
          <statement>
            <p>
              Prove the reduction formula
              <me>
                \int \cos^nx\,dx = \frac{1}{n} \cos^{n-1}x \sin x + \frac{n-1}{n}\int\cos^{n-2}x\,dx.
              </me>
            </p>
          </statement>

          <hint>
            <p>
              You are going to integrate <em>something</em> by parts.
              How can you break up <m>\cos^n x\,dx</m> into <m>u \,dv</m> that makes <m>dv</m> easily to integrate?
            </p>
          </hint>
        </exercise>
      </page>
    </worksheet>
  </article>
</pretext>