<?xml version="1.0" encoding="UTF-8" ?>
<!-- Generated by Pandoc using pretext.lua -->
<pretext>
<article>



	<section xml:id="basic-forms" class="unnumbered">
		<title>BASIC FORMS</title>

		<p><ol>
			<li>
					<p>
						<m>\int u d v=u v-\int v d u</m>
					</p>
			</li>

			<li>
					<p>
						<m>\int u^{n} d u=\frac{u^{n+1}}{n+1}+C, \quad n \neq-1</m>
					</p>
			</li>

			<li>
					<p>
						<m>\int \frac{d u}{u}=\ln |u|+C</m>
					</p>
			</li>

			<li>
					<p>
						<m>\int e^{u} d u=e^{u}+C</m>
					</p>
			</li>

			<li>
					<p>
						<m>\int a^{u} d u=\frac{a^{u}}{\ln a}+C</m>
					</p>
			</li>

			<li>
					<p>
						<m>\int \sin u d u=-\cos u+C</m>
					</p>
			</li>

			<li>
					<p>
						<m>\int \cos u d u=\sin u+C</m>
					</p>
			</li>

			<li>
					<p>
						<m>\int \sec ^{2} u d u=\tan u+C</m>
					</p>
			</li>

			<li>
					<p>
						<m>\int \csc ^{2} u d u=-\cot u+C</m>
					</p>
			</li>

			<li>
					<p>
						<m>\int \sec u \tan u d u=\sec u+C</m>
					</p>
			</li>

			<li>
					<p>
						<m>\int \csc u \cot u d u=-\csc u+C</m>
					</p>
			</li>

			<li>
					<p>
						<m>\int \tan u d u=\ln |\sec u|+C</m>
					</p>
			</li>

			<li>
					<p>
						<m>\int \cot u d u=\ln |\sin u|+C</m>
					</p>
			</li>

			<li>
					<p>
						<m>\int \sec u d u=\ln |\sec u+\tan u|+C</m>
					</p>
			</li>

			<li>
					<p>
						<m>\int \csc u d u=\ln |\csc u-\cot u|+C</m>
					</p>
			</li>

			<li>
					<p>
						<m>\int \frac{d u}{\sqrt{a^{2}-u^{2}}}=\sin ^{-1} \frac{u}{a}+C, \quad a&gt;0</m>
					</p>
			</li>

			<li>
					<p>
						<m>\int \frac{d u}{a^{2}+u^{2}}=\frac{1}{a} \tan ^{-1} \frac{u}{a}+C</m>
					</p>
			</li>

			<li>
					<p>
						<m>\int \frac{d u}{u \sqrt{u^{2}-a^{2}}}=\frac{1}{a} \sec ^{-1} \frac{u}{a}+C</m>
					</p>
			</li>

			<li>
					<p>
						<m>\int \frac{d u}{a^{2}-u^{2}}=\frac{1}{2 a} \ln \left|\frac{u+a}{u-a}\right|+C</m>
					</p>
			</li>

			<li>
					<p>
						<m>\int \frac{d u}{u^{2}-a^{2}}=\frac{1}{2 a} \ln \left|\frac{u-a}{u+a}\right|+C</m>
					</p>
			</li>

		</ol></p>

	</section>

	<section xml:id="forms-involving-sqrta2u2-a0" class="unnumbered">
		<title>FORMS INVOLVING <m>\sqrt{a^{2}+u^{2}}, a&gt;0</m></title>

		<p><ol>
			<li>
					<p>
						<m>\int \sqrt{a^{2}+u^{2}} d u=\frac{u}{2} \sqrt{a^{2}+u^{2}}+\frac{a^{2}}{2} \ln \left(u+\sqrt{a^{2}+u^{2}}\right)+C</m>
					</p>
			</li>

			<li>
					<p>
						<m>\int u^{2} \sqrt{a^{2}+u^{2}} d u=\frac{u}{8}\left(a^{2}+2 u^{2}\right) \sqrt{a^{2}+u^{2}}-\frac{a^{4}}{8} \ln \left(u+\sqrt{a^{2}+u^{2}}\right)+C</m>
					</p>
			</li>

			<li>
					<p>
						<m>\int \frac{\sqrt{a^{2}+u^{2}}}{u} d u=\sqrt{a^{2}+u^{2}}-a \ln \left|\frac{a+\sqrt{a^{2}+u^{2}}}{u}\right|+C</m>
					</p>
			</li>

			<li>
					<p>
						<m>\int \frac{\sqrt{a^{2}+u^{2}}}{u^{2}} d u=-\frac{\sqrt{a^{2}+u^{2}}}{u}+\ln \left(u+\sqrt{a^{2}+u^{2}}\right)+C</m>
					</p>
			</li>

			<li>
					<p>
						<m>\int \frac{d u}{\sqrt{a^{2}+u^{2}}}=\ln \left(u+\sqrt{a^{2}+u^{2}}\right)+C</m>
					</p>
			</li>

			<li>
					<p>
						<m>\int \frac{u^{2} d u}{\sqrt{a^{2}+u^{2}}}=\frac{u}{2} \sqrt{a^{2}+u^{2}}-\frac{a^{2}}{2} \ln \left(u+\sqrt{a^{2}+u^{2}}\right)+C</m>
					</p>
			</li>

			<li>
					<p>
						<m>\int \frac{d u}{u \sqrt{a^{2}+u^{2}}}=-\frac{1}{a} \ln \left|\frac{\sqrt{a^{2}+u^{2}}+a}{u}\right|+C</m>
					</p>
			</li>

			<li>
					<p>
						<m>\int \frac{d u}{u^{2} \sqrt{a^{2}+u^{2}}}=-\frac{\sqrt{a^{2}+u^{2}}}{a^{2} u}+C</m>
					</p>
			</li>

			<li>
					<p>
						<m>\int \frac{d u}{\left(a^{2}+u^{2}\right)^{3 / 2}}=\frac{u}{a^{2} \sqrt{a^{2}+u^{2}}}+C</m>
					</p>
			</li>

		</ol></p>

		<p>
			FORMS INVOLVING <m>\sqrt{a^{2}-u^{2}}, a&gt;0</m><!-- linebreak -->30. <m>\int \sqrt{a^{2}-u^{2}} d u=\frac{u}{2} \sqrt{a^{2}-u^{2}}+\frac{a^{2}}{2} \sin ^{-1} \frac{u}{a}+C</m><!-- linebreak -->31. <m>\int u^{2} \sqrt{a^{2}-u^{2}} d u=\frac{u}{8}\left(2 u^{2}-a^{2}\right) \sqrt{a^{2}-u^{2}}+\frac{a^{4}}{8} \sin ^{-1} \frac{u}{a}+C</m><!-- linebreak -->32. <m>\int \frac{\sqrt{a^{2}-u^{2}}}{u} d u=\sqrt{a^{2}-u^{2}}-a \ln \left|\frac{a+\sqrt{a^{2}-u^{2}}}{u}\right|+C</m><!-- linebreak -->33. <m>\int \frac{\sqrt{a^{2}-u^{2}}}{u^{2}} d u=-\frac{1}{u} \sqrt{a^{2}-u^{2}}-\sin ^{-1} \frac{u}{a}+C</m><!-- linebreak -->34. <m>\int \frac{u^{2} d u}{\sqrt{a^{2}-u^{2}}}=-\frac{u}{2} \sqrt{a^{2}-u^{2}}+\frac{a^{2}}{2} \sin ^{-1} \frac{u}{a}+C</m><!-- linebreak -->35. <m>\int \frac{d u}{u \sqrt{a^{2}-u^{2}}}=-\frac{1}{a} \ln \left|\frac{a+\sqrt{a^{2}-u^{2}}}{u}\right|+C</m><!-- linebreak -->36. <m>\int \frac{d u}{u^{2} \sqrt{a^{2}-u^{2}}}=-\frac{1}{a^{2} u} \sqrt{a^{2}-u^{2}}+C</m><!-- linebreak -->37. <m>\int\left(a^{2}-u^{2}\right)^{3 / 2} d u=-\frac{u}{8}\left(2 u^{2}-5 a^{2}\right) \sqrt{a^{2}-u^{2}}+\frac{3 a^{4}}{8} \sin ^{-1} \frac{u}{a}+C</m><!-- linebreak -->38. <m>\int \frac{d u}{\left(a^{2}-u^{2}\right)^{3 / 2}}=\frac{u}{a^{2} \sqrt{a^{2}-u^{2}}}+C</m>
		</p>

		<p>
			FORMS INVOLVING <m>\sqrt{u^{2}-a^{2}}, a&gt;0</m><!-- linebreak -->39. <m>\int \sqrt{u^{2}-a^{2}} d u=\frac{u}{2} \sqrt{u^{2}-a^{2}}-\frac{a^{2}}{2} \ln \left|u+\sqrt{u^{2}-a^{2}}\right|+C</m><!-- linebreak -->40. <m>\int u^{2} \sqrt{u^{2}-a^{2}} d u=\frac{u}{8}\left(2 u^{2}-a^{2}\right) \sqrt{u^{2}-a^{2}}-\frac{a^{4}}{8} \ln \left|u+\sqrt{u^{2}-a^{2}}\right|+C</m><!-- linebreak -->41. <m>\int \frac{\sqrt{u^{2}-a^{2}}}{u} d u=\sqrt{u^{2}-a^{2}}-a \cos ^{-1} \frac{a}{|u|}+C</m><!-- linebreak -->42. <m>\int \frac{\sqrt{u^{2}-a^{2}}}{u^{2}} d u=-\frac{\sqrt{u^{2}-a^{2}}}{u}+\ln \left|u+\sqrt{u^{2}-a^{2}}\right|+C</m><!-- linebreak -->43. <m>\int \frac{d u}{\sqrt{u^{2}-a^{2}}}=\ln \left|u+\sqrt{u^{2}-a^{2}}\right|+C</m><!-- linebreak -->44. <m>\int \frac{u^{2} d u}{\sqrt{u^{2}-a^{2}}}=\frac{u}{2} \sqrt{u^{2}-a^{2}}+\frac{a^{2}}{2} \ln \left|u+\sqrt{u^{2}-a^{2}}\right|+C</m><!-- linebreak -->45. <m>\int \frac{d u}{u^{2} \sqrt{u^{2}-a^{2}}}=\frac{\sqrt{u^{2}-a^{2}}}{a^{2} u}+C</m><!-- linebreak -->46. <m>\int \frac{d u}{\left(u^{2}-a^{2}\right)^{3 / 2}}=-\frac{u}{a^{2} \sqrt{u^{2}-a^{2}}}+C</m>
		</p>

	</section>

	<section xml:id="forms-involving-ab-u" class="unnumbered">
		<title>FORMS INVOLVING <m>a+b u</m></title>

		<p><ol>
			<li>
					<p>
						<m>\int \frac{u d u}{a+b u}=\frac{1}{b^{2}}(a+b u-a \ln |a+b u|)+C</m>
					</p>
			</li>

			<li>
					<p>
						<m>\int \frac{u^{2} d u}{a+b u}=\frac{1}{2 b^{3}}\left[(a+b u)^{2}-4 a(a+b u)+2 a^{2} \ln |a+b u|\right]+C</m>
					</p>
			</li>

			<li>
					<p>
						<m>\int \frac{d u}{u(a+b u)}=\frac{1}{a} \ln \left|\frac{u}{a+b u}\right|+C</m>
					</p>
			</li>

			<li>
					<p>
						<m>\int \frac{d u}{u^{2}(a+b u)}=-\frac{1}{a u}+\frac{b}{a^{2}} \ln \left|\frac{a+b u}{u}\right|+C</m>
					</p>
			</li>

			<li>
					<p>
						<m>\int \frac{u d u}{(a+b u)^{2}}=\frac{a}{b^{2}(a+b u)}+\frac{1}{b^{2}} \ln |a+b u|+C</m>
					</p>
			</li>

			<li>
					<p>
						<m>\int \frac{d u}{u(a+b u)^{2}}=\frac{1}{a(a+b u)}-\frac{1}{a^{2}} \ln \left|\frac{a+b u}{u}\right|+C</m>
					</p>
			</li>

			<li>
					<p>
						<m>\int \frac{u^{2} d u}{(a+b u)^{2}}=\frac{1}{b^{3}}\left(a+b u-\frac{a^{2}}{a+b u}-2 a \ln |a+b u|\right)+C</m>
					</p>
			</li>

			<li>
					<p>
						<m>\int u \sqrt{a+b u} d u=\frac{2}{15 b^{2}}(3 b u-2 a)(a+b u)^{3 / 2}+C</m>
					</p>
			</li>

			<li>
					<p>
						<m>\int \frac{u d u}{\sqrt{a+b u}}=\frac{2}{3 b^{2}}(b u-2 a) \sqrt{a+b u}+C</m>
					</p>
			</li>

			<li>
					<p>
						<m>\int \frac{u^{2} d u}{\sqrt{a+b u}}=\frac{2}{15 b^{3}}\left(8 a^{2}+3 b^{2} u^{2}-4 a b u\right) \sqrt{a+b u}+C</m>
					</p>
			</li>

			<li>
					<p>
						<m>\int \frac{d u}{u \sqrt{a+b u}}=\frac{1}{\sqrt{a}} \ln \left|\frac{\sqrt{a+b u}-\sqrt{a}}{\sqrt{a+b u}+\sqrt{a}}\right|+C, \quad</m> if <m>a&gt;0</m>
					</p>
			</li>

		</ol></p>

		<p>
			<me>=\frac{2}{\sqrt{-a}} \tan ^{-1} \sqrt{\frac{a+b u}{-a}}+C, \quad \text { if } a&lt;0</me>
		</p>

		<p><ol>
			<li>
					<p>
						<m>\int \frac{\sqrt{a+b u}}{u} d u=2 \sqrt{a+b u}+a \int \frac{d u}{u \sqrt{a+b u}}</m>
					</p>
			</li>

			<li>
					<p>
						<m>\int \frac{\sqrt{a+b u}}{u^{2}} d u=-\frac{\sqrt{a+b u}}{u}+\frac{b}{2} \int \frac{d u}{u \sqrt{a+b u}}</m>
					</p>
			</li>

			<li>
					<p>
						<m>\int u^{n} \sqrt{a+b u} d u=\frac{2}{b(2 n+3)}\left[u^{n}(a+b u)^{3 / 2}-n a \int u^{n-1} \sqrt{a+b u} d u\right]</m>
					</p>
			</li>

			<li>
					<p>
						<m>\int \frac{u^{n} d u}{\sqrt{a+b u}}=\frac{2 u^{n} \sqrt{a+b u}}{b(2 n+1)}-\frac{2 n a}{b(2 n+1)} \int \frac{u^{n-1} d u}{\sqrt{a+b u}}</m>
					</p>
			</li>

			<li>
					<p>
						<m>\int \frac{d u}{u^{n} \sqrt{a+b u}}=-\frac{\sqrt{a+b u}}{a(n-1) u^{n-1}}-\frac{b(2 n-3)}{2 a(n-1)} \int \frac{d u}{u^{n-1} \sqrt{a+b u}}</m>
					</p>
			</li>

		</ol></p>

	</section>

	<section xml:id="inverse-trigonometric-forms" class="unnumbered">
		<title>INVERSE TRIGONOMETRIC FORMS</title>

		<p><ol>
			<li>
					<p>
						<m>\int \sin ^{-1} u d u=u \sin ^{-1} u+\sqrt{1-u^{2}}+C</m>
					</p>
			</li>

			<li>
					<p>
						<m>\int \cos ^{-1} u d u=u \cos ^{-1} u-\sqrt{1-u^{2}}+C</m>
					</p>
			</li>

			<li>
					<p>
						<m>\int \tan ^{-1} u d u=u \tan ^{-1} u-\frac{1}{2} \ln \left(1+u^{2}\right)+C</m>
					</p>
			</li>

			<li>
					<p>
						<m>\int u \sin ^{-1} u d u=\frac{2 u^{2}-1}{4} \sin ^{-1} u+\frac{u \sqrt{1-u^{2}}}{4}+C</m>
					</p>
			</li>

			<li>
					<p>
						<m>\int u \cos ^{-1} u d u=\frac{2 u^{2}-1}{4} \cos ^{-1} u-\frac{u \sqrt{1-u^{2}}}{4}+C</m>
					</p>
			</li>

			<li>
					<p>
						<m>\int u \tan ^{-1} u d u=\frac{u^{2}+1}{2} \tan ^{-1} u-\frac{u}{2}+C</m>
					</p>
			</li>

			<li>
					<p>
						<m>\int u^{n} \sin ^{-1} u d u=\frac{1}{n+1}\left[u^{n+1} \sin ^{-1} u-\int \frac{u^{n+1} d u}{\sqrt{1-u^{2}}}\right], \quad n \neq-1</m>
					</p>
			</li>

			<li>
					<p>
						<m>\int u^{n} \cos ^{-1} u d u=\frac{1}{n+1}\left[u^{n+1} \cos ^{-1} u+\int \frac{u^{n+1} d u}{\sqrt{1-u^{2}}}\right], \quad n \neq-1</m>
					</p>
			</li>

			<li>
					<p>
						<m>\int u^{n} \tan ^{-1} u d u=\frac{1}{n+1}\left[u^{n+1} \tan ^{-1} u-\int \frac{u^{n+1} d u}{1+u^{2}}\right], \quad n \neq-1</m>
					</p>
			</li>

		</ol></p>

	</section>

	<section xml:id="trigonometric-forms" class="unnumbered">
		<title>TRIGONOMETRIC FORMS</title>

		<p><ol>
			<li>
					<p>
						<m>\int \cot ^{n} u d u=\frac{-1}{n-1} \cot ^{n-1} u-\int \cot ^{n-2} u d u</m>
					</p>
			</li>

			<li>
					<p>
						<m>\int \sec ^{n} u d u=\frac{1}{n-1} \tan u \sec ^{n-2} u+\frac{n-2}{n-1} \int \sec ^{n-2} u d u</m>
					</p>
			</li>

			<li>
					<p>
						<m>\int \csc ^{n} u d u=\frac{-1}{n-1} \cot u \csc ^{n-2} u+\frac{n-2}{n-1} \int \csc ^{n-2} u d u</m>
					</p>
			</li>

			<li>
					<p>
						<m>\int \sin a u \sin b u d u=\frac{\sin (a-b) u}{2(a-b)}-\frac{\sin (a+b) u}{2(a+b)}+C</m>
					</p>
			</li>

			<li>
					<p>
						<m>\int \cos a u \cos b u d u=\frac{\sin (a-b) u}{2(a-b)}+\frac{\sin (a+b) u}{2(a+b)}+C</m>
					</p>
			</li>

			<li>
					<p>
						<m>\int \sin a u \cos b u d u=-\frac{\cos (a-b) u}{2(a-b)}-\frac{\cos (a+b) u}{2(a+b)}+C</m>
					</p>
			</li>

			<li>
					<p>
						<m>\int u \sin u d u=\sin u-u \cos u+C</m>
					</p>
			</li>

			<li>
					<p>
						<m>\int u \cos u d u=\cos u+u \sin u+C</m>
					</p>
			</li>

			<li>
					<p>
						<m>\int u^{n} \sin u d u=-u^{n} \cos u+n \int u^{n-1} \cos u d u</m>
					</p>
			</li>

			<li>
					<p>
						<m>\int u^{n} \cos u d u=u^{n} \sin u-n \int u^{n-1} \sin u d u</m>
					</p>
			</li>

			<li>
					<p>
						<m>\int \sin ^{n} u \cos ^{m} u d u=-\frac{\sin ^{n-1} u \cos ^{m+1} u}{n+m}+\frac{n-1}{n+m} \int \sin ^{n-2} u \cos ^{m} u d u</m> <m>=\frac{\sin ^{n+1} u \cos ^{m-1} u}{n+m}+\frac{m-1}{n+m} \int \sin ^{n} u \cos ^{m-2} u d u</m><!-- linebreak --><m>=\frac{\sin ^{n+1} u \cos ^{m-1} u}{n+m}+\frac{m-1}{n+m} \int</m>
					</p>
			</li>

		</ol></p>

		<p>
			<me>\overline{n+m}+\overline{n+m}</me>
		</p>

		<p><ol>
			<li>
					<p>
						<m>\int \sin ^{2} u d u=\frac{1}{2} u-\frac{1}{4} \sin 2 u+C</m>
					</p>
			</li>

			<li>
					<p>
						<m>\int \cos ^{2} u d u=\frac{1}{2} u+\frac{1}{4} \sin 2 u+C</m>
					</p>
			</li>

			<li>
					<p>
						<m>\int \tan ^{2} u d u=\tan u-u+C</m>
					</p>
			</li>

			<li>
					<p>
						<m>\int \cot ^{2} u d u=-\cot u-u+C</m>
					</p>
			</li>

			<li>
					<p>
						<m>\int \sin ^{3} u d u=-\frac{1}{3}\left(2+\sin ^{2} u\right) \cos u+C</m>
					</p>
			</li>

			<li>
					<p>
						<m>\int \cos ^{3} u d u=\frac{1}{3}\left(2+\cos ^{2} u\right) \sin u+C</m>
					</p>
			</li>

			<li>
					<p>
						<m>\int \tan ^{3} u d u=\frac{1}{2} \tan ^{2} u+\ln |\cos u|+C</m>
					</p>
			</li>

			<li>
					<p>
						<m>\int \cot ^{3} u d u=-\frac{1}{2} \cot ^{2} u-\ln |\sin u|+C</m>
					</p>
			</li>

			<li>
					<p>
						<m>\int \sec ^{3} u d u=\frac{1}{2} \sec u \tan u+\frac{1}{2} \ln |\sec u+\tan u|+C</m>
					</p>
			</li>

			<li>
					<p>
						<m>\int \csc ^{3} u d u=-\frac{1}{2} \csc u \cot u+\frac{1}{2} \ln |\csc u-\cot u|+C</m>
					</p>
			</li>

			<li>
					<p>
						<m>\int \sin ^{n} u d u=-\frac{1}{n} \sin ^{n-1} u \cos u+\frac{n-1}{n} \int \sin ^{n-2} u d u</m>
					</p>
			</li>

			<li>
					<p>
						<m>\int \cos ^{n} u d u=\frac{1}{n} \cos ^{n-1} u \sin u+\frac{n-1}{n} \int \cos ^{n-2} u d u</m>
					</p>
			</li>

			<li>
					<p>
						<m>\int \tan ^{n} u d u=\frac{1}{n-1} \tan ^{n-1} u-\int \tan ^{n-2} u d u</m>
					</p>
			</li>

		</ol></p>
	</section>



</article>
</pretext>
