<?xml version="1.0" encoding="UTF-8"?>
<pretext xmlns:xi="http://www.w3.org/2001/XInclude">
  <article>
    <section xml:id="ps03-section">
      <title>Problem Set 3</title>
      <subtitle>Trigonometric Substitution and Partial Fractions </subtitle>
      <introduction>
        <p>
          This problem set consists not only of problems similar to what you've seen, but
          also of unique problems you may not have seen before.
          The purpose is for you to apply the concepts you've previously
          learned to new, unfamiliar, and usually more interesting situations.
          In some cases, problems connect ideas from multiple learning objectives.
        </p>

        <p> Write full, clear solutions to the problems below. Although the final answer is
          important, being able to convey you understand the underlying concepts is more important.
          So show your work and explain your steps. Write complete sentences in English to connect
          your mathematical statements. Do not use the three-dots notation (∴ or ∵) when you mean <q>
          therefore</q> or <q>because</q>. Do not use an arrow (→) when you mean equals (=) or <q>this
          implies</q> or <q>and now the next step is…</q>. Use the worked examples in the textbook, or
          on solution sets to worksheets or previous problem sets, as a guide for how to write your
          solutions. </p>

        <p>Written work should be neat and legible.
          Other than being written in longhand, your work should be as clean as something you would
          turn in for one of your writing classes.
          Write in linear order from left to right and top to bottom.
          Leave ample space for graders to write their comments.
          (Do not upload the exercise sheet with your answers written in the margins.)
          Setting aside one page per exercise is a good rule of thumb.
        </p>

        <p>
          Prepare a single PDF and submit it to Gradescope.
          Mark the page of each exercise when you upload your pset.
          Make sure each page is in the proper orientation.
        </p>

      </introduction>
      <exercises>
        <exercise xml:id="ex-trig-sub-definite-x-squared-plus-four">
          <statement>
            <p> Evaluate the definite integral <me>\int_1^3 \frac{dx}{x^2\sqrt{x^2+4}}</me>. Explain
              your steps and justify your choices for trigonometric substitution. </p>
          </statement>
          <solution>
            <p> The form <m>\sqrt{x^2+a^2}</m> suggests a tangent substitution. Let <m>x =
              2\tan\theta</m>. Then <m>dx = 2\sec^2\theta \,d\theta</m>. </p>
            <p> The square root becomes <m>\sqrt{(2\tan\theta)^2+4} = \sqrt{4\tan^2\theta+4} =
              \sqrt{4(\tan^2\theta+1)} = \sqrt{4\sec^2\theta} = 2\sec\theta</m>. </p>
            <p> We must also change the limits of integration. When <m>x=1</m>, <m>1 = 2\tan\theta</m>,
              so <m>\theta = \arctan(1/2)</m>. When <m>x=3</m>, <m>3 = 2\tan\theta</m>, so <m>\theta
              = \arctan(3/2)</m>. </p>
            <p>
              Substitute these into the integral:
            </p>
            <me>
              \int_{\arctan(1/2)}^{\arctan(3/2)} \frac{2\sec^2\theta \,d\theta}{(2\tan\theta)^2
              (2\sec\theta)}
            </me>
            <me>
              = \int_{\arctan(1/2)}^{\arctan(3/2)} \frac{2\sec^2\theta}{4\tan^2\theta \cdot
              2\sec\theta} \,d\theta
            </me>
            <me>
              = \frac{1}{4} \int_{\arctan(1/2)}^{\arctan(3/2)} \frac{\sec\theta}{\tan^2\theta}
              \,d\theta
            </me>
            <p>
              Convert to sine and cosine:
            </p>
            <me>
              \frac{1}{4} \int \frac{1/\cos\theta}{\sin^2\theta/\cos^2\theta} \,d\theta =
              \frac{1}{4} \int \frac{\cos\theta}{\sin^2\theta} \,d\theta
            </me>
            <p> Let <m>u = \sin\theta</m>, so <m>du = \cos\theta \,d\theta</m>. </p>
            <me>
              = \frac{1}{4} \int u^{-2} \,du = \frac{1}{4} \left( -u^{-1} \right) =
              -\frac{1}{4\sin\theta} = -\frac{1}{4}\csc\theta
            </me>
            <p> We can now evaluate the definite integral using our new limits and the fact that <m>\csc\theta
              = \frac{\text{hypotenuse}}{\text{opposite}}</m>. For <m>\theta = \arctan(3/2)</m>,
              consider a right triangle with opposite side 3 and adjacent side 2. The hypotenuse is <m>\sqrt{3^2+2^2}
              = \sqrt{13}</m>. So, <m>\csc(\arctan(3/2)) = \sqrt{13}/3</m>. For <m>\theta =
              \arctan(1/2)</m>, consider a right triangle with opposite side 1 and adjacent side 2.
              The hypotenuse is <m>\sqrt{1^2+2^2} = \sqrt{5}</m>. So, <m>\csc(\arctan(1/2)) =
              \sqrt{5}/1 = \sqrt{5}</m>. </p>
            <me>
              \left[ -\frac{1}{4}\csc\theta \right]_{\arctan(1/2)}^{\arctan(3/2)} =
              -\frac{1}{4}\left(\frac{\sqrt{13}}{3} - \sqrt{5}\right) = \frac{\sqrt{5}}{4} -
              \frac{\sqrt{13}}{12}
            </me>
          </solution>
        </exercise>

        <exercise xml:id="ex-trig-sub-completing-the-square">
          <statement>
            <p> Evaluate the indefinite integral <me>\int \frac{x^2}{\sqrt{4x-x^2}} \,dx</me>. </p>
          </statement>
          <solution>
            <p> This problem requires completing the square before using trigonometric substitution. <me>
              4x-x^2 = -(x^2-4x) = -(x^2-4x+4-4) = 4-(x-2)^2
              </me>
            </p>
            <p> The integral becomes <me>\int \frac{x^2}{\sqrt{4-(x-2)^2}} \,dx</me>. The form <m>
              \sqrt{a^2-u^2}</m> suggests a sine substitution. Let <m>u = x-2</m>. Then <m>x = u+2</m>
              and <m>dx = du</m>. The integral is now <me>\int \frac{(u+2)^2}{\sqrt{4-u^2}} \,du</me>
              . </p>
            <p> Now, let <m>u = 2\sin\theta</m>. Then <m>du = 2\cos\theta \,d\theta</m>. Also, <m>\sqrt{4-u^2}
              = \sqrt{4-4\sin^2\theta} = \sqrt{4\cos^2\theta} = 2\cos\theta</m>. </p>
            <p>
              Substitute these into the integral:
            </p>
            <me>
              \int \frac{(2\sin\theta+2)^2}{2\cos\theta} (2\cos\theta) \,d\theta = \int
              (2\sin\theta+2)^2 \,d\theta
            </me>
            <me>
              = \int (4\sin^2\theta+8\sin\theta+4) \,d\theta
            </me>
            <p> Use the half-angle identity <m>\sin^2\theta = \frac{1-\cos(2\theta)}{2}</m>: </p>
            <me>
              = \int \left(4\left(\frac{1-\cos(2\theta)}{2}\right) + 8\sin\theta + 4\right)
              \,d\theta
            </me>
            <me>
              = \int (2-2\cos(2\theta) + 8\sin\theta + 4) \,d\theta = \int (6 - 2\cos(2\theta) +
              8\sin\theta) \,d\theta
            </me>
            <me>
              = 6\theta - \sin(2\theta) - 8\cos\theta + C
            </me>
            <p> Since <m>\sin(2\theta) = 2\sin\theta\cos\theta</m>, we have <m>6\theta -
              2\sin\theta\cos\theta - 8\cos\theta + C</m>. </p>
            <p> We need to substitute back in terms of <m>x</m>. From <m>u = 2\sin\theta</m>, we get <m>\sin\theta
              = u/2</m>. Draw a right triangle to find <m>\cos\theta = \frac{\sqrt{4-u^2}}{2}</m>
              and <m>\theta = \arcsin(u/2)</m>. </p>
            <me>
              = 6\arcsin\left(\frac{u}{2}\right) -
              2\left(\frac{u}{2}\right)\left(\frac{\sqrt{4-u^2}}{2}\right) -
              8\left(\frac{\sqrt{4-u^2}}{2}\right) + C
            </me>
            <me>
              = 6\arcsin\left(\frac{u}{2}\right) - \frac{u\sqrt{4-u^2}}{2} - 4\sqrt{4-u^2} + C
            </me>
            <p> Finally, substitute back <m>u=x-2</m> to get the final answer in terms of <m>x</m>. </p>
          </solution>
        </exercise>

        <exercise xml:id="ex-partial-fractions-long-division">
          <statement>
            <p> Evaluate the indefinite integral <me>\int \frac{x^3-4x-10}{x^2-x-6} \,dx</me>. </p>
          </statement>
          <solution>
            <p>
              Since the degree of the numerator is greater than the degree of the denominator, we
              must perform long division first.
            </p>
            <me>
              \frac{x^3-4x-10}{x^2-x-6} = x+1 + \frac{3x-4}{x^2-x-6}
            </me>
            <p> So the integral becomes <me>\int \left( x+1 + \frac{3x-4}{x^2-x-6} \right) \,dx</me>.
              We now use partial fractions on the remaining rational function. Factor the
              denominator: <m>x^2-x-6 = (x-3)(x+2)</m>. </p>
            <me>
              \frac{3x-4}{(x-3)(x+2)} = \frac{A}{x-3} + \frac{B}{x+2}
            </me>
            <p> Multiply both sides by <m>(x-3)(x+2)</m>: <me>
                3x-4 = A(x+2) + B(x-3)
              </me> To solve for <m>A</m>, let <m>
              x=3</m>: <m>3(3)-4 = A(3+2) \implies 5 = 5A \implies A=1</m>. To solve for <m>B</m>,
              let <m>x=-2</m>: <m>3(-2)-4 = B(-2-3) \implies -10 = -5B \implies B=2</m>. </p>
            <p> The partial fraction decomposition is <me>\frac{1}{x-3} + \frac{2}{x+2}</me>. </p>
            <p>
              Now we integrate:
            </p>
            <me>
              \int \left( x+1 + \frac{1}{x-3} + \frac{2}{x+2} \right) \,dx
            </me>
            <me>
              = \frac{1}{2}x^2 + x + \ln|x-3| + 2\ln|x+2| + C
            </me>
          </solution>
        </exercise>

        <exercise xml:id="ex-trig-sub-one-over-x-sqrt">
          <statement>
            <p> Evaluate the indefinite integral <me>\int \frac{1}{x\sqrt{4-x^2}} \,dx</me>. </p>
          </statement>
          <solution>
            <p> The form <m>\sqrt{a^2-x^2}</m> suggests a sine substitution. Let <m>x = 2\sin\theta</m>.
              Then <m>dx = 2\cos\theta \,d\theta</m>. </p>
            <p> The square root becomes <m>\sqrt{4-(2\sin\theta)^2} = \sqrt{4-4\sin^2\theta} =
              \sqrt{4\cos^2\theta} = 2\cos\theta</m>. </p>
            <p>
              Substitute these into the integral:
            </p>
            <me>
              \int \frac{2\cos\theta \,d\theta}{(2\sin\theta)(2\cos\theta)}
            </me>
            <me>
              = \int \frac{1}{2\sin\theta} \,d\theta = \frac{1}{2}\int \csc\theta \,d\theta
            </me>
            <p> The integral of cosecant is a standard result: <m>\int \csc\theta \,d\theta =
              \ln|\csc\theta - \cot\theta|</m>. </p>
            <me>
              = \frac{1}{2}\ln|\csc\theta - \cot\theta| + C
            </me>
            <p> To substitute back in terms of <m>x</m>, we use a right triangle. Since <m>\sin\theta
              = x/2</m>, the opposite side is <m>x</m> and the hypotenuse is 2. The adjacent side is <m>
              \sqrt{4-x^2}</m>. </p>
            <me>
              \csc\theta = \frac{2}{x}
            </me>
            <me>
              \cot\theta = \frac{\sqrt{4-x^2}}{x}
            </me>
            <p>
              Substitute these back into the expression:
            </p>
            <me>
              = \frac{1}{2}\ln\left|\frac{2}{x} - \frac{\sqrt{4-x^2}}{x}\right| + C
            </me>
            <me>
              = \frac{1}{2}\ln\left|\frac{2 - \sqrt{4-x^2}}{x}\right| + C
            </me>
          </solution>
        </exercise>
        <exercise xml:id="ex-partial-fractions-repeated-quadratic">
          <statement>
            <p> Evaluate the definite integral <me>\int_{0}^{1/\sqrt{3}} \frac{x}{(x-1)^2(x^2+1)}
              \,dx</me>. </p>
          </statement>
          <solution>
            <p>
              The denominator has a repeated linear factor and an irreducible quadratic factor.
              The form of the partial fraction decomposition is:
            </p>
            <me>
              \frac{x}{(x-1)^2(x^2+1)} = \frac{A}{x-1} + \frac{B}{(x-1)^2} + \frac{Cx+D}{x^2+1}
            </me>
            <p> Multiply by the denominator: <me>
                x = A(x-1)(x^2+1) + B(x^2+1) + (Cx+D)(x-1)^2
              </me> To
              solve for <m>B</m>, let <m>x=1</m>: <m>1 = B(1^2+1) \implies 1 = 2B \implies B =
              \frac{1}{2}</m>. </p>
            <p> Now expand and collect powers of <m>x</m> to find <m>A, C, D</m>. <me>
                x = A(x^3-x^2+x-1) + B(x^2+1) + (Cx+D)(x^2-2x+1)
              </me>
              <me>
              x = Ax^3-Ax^2+Ax-A + Bx^2+B + Cx^3-2Cx^2+Cx + Dx^2-2Dx+D
              </me>
              <me>
              x = (A+C)x^3 + (-A+B-2C+D)x^2 + (A+C-2D)x + (-A+B+D)
              </me>
            </p>
            <p> Comparing coefficients: <me>
                x^3: A+C = 0 \implies C = -A
              </me>
              <me>
                x^2: -A+B-2C+D = 0
              </me>
              <me>
                x^1: A+C-2D = 1
              </me>
              <me>
                x^0: -A+B+D = 0
              </me>
            </p>
            <p> From <m>A+C=0</m> and <m>A+C-2D=1</m>, we get <m>0-2D=1 \implies D = -\frac{1}{2}</m>.
              Now use <m>-A+B+D=0</m> with <m>B=1/2</m> and <m>D=-1/2</m>: <m>-A + \frac{1}{2} -
              \frac{1}{2} = 0 \implies A=0</m>. From <m>C=-A</m>, we have <m>C=0</m>. </p>
            <p> The decomposition is <me>\frac{1/2}{(x-1)^2} + \frac{-1/2}{x^2+1}</me>. </p>
            <me>
              \int \left( \frac{1}{2(x-1)^2} - \frac{1}{2(x^2+1)} \right) \,dx
            </me>
            <me>
              = -\frac{1}{2(x-1)} - \frac{1}{2}\arctan(x) + C
            </me>
            <p> Now we evaluate the definite integral from 0 to <m>1/\sqrt{3}</m>. <md>
                <mrow> \int_{0}^{1/\sqrt{3}} \frac{x}{(x-1)^2(x^2+1)} \,dx
                  \amp = \left[-\frac{1}{2(x-1)} - \frac{1}{2}\arctan(x) \right]_0^{\pi/3}</mrow>
                <mrow> \amp = \frac{1}{2}\left[\frac{1}{x-1} + \arctan(x) \right]^0_{\pi/3}</mrow>
                <mrow> \amp = \frac{1}{2}\left[
                  \left(\frac{1}{-1} + \frac{1}{2}\arctan(0)\right) -
                  \left(\frac{1}{\sqrt{3}-1} + \arctan\left(1/\sqrt{3}\right)\right) \right]
                </mrow>
                <mrow> \amp = \frac{1}{2}\left[
                  \left(-1 + 0 \right) -
                  \left(\frac{\sqrt{3}}{1-\sqrt{3}} + \frac{\pi}{6}\right) \right]
                </mrow>
                <mrow> \amp = \frac{1}{2}\left[
                  -1 + \frac{\sqrt{3}}{\sqrt{3}-1} - \frac{\pi}{6} \right]
                </mrow>
                <mrow> \amp = \frac{\sqrt{3}}{2\sqrt{3}-2)} - \frac{\pi}{12} - \frac{1}{2}
                </mrow>
              </md>
            </p>
          </solution>
        </exercise>

        <exercise xml:id="ex-partial-fractions-u-sub">
          <statement>
            <p> Evaluate the indefinite integral <me>\int \frac{1}{e^{2x}-e^x-2} \,dx</me>. </p>
          </statement>
          <solution>
            <p> This problem requires a substitution before partial fractions can be used. Let <m>u
                = e^x</m>. Then <m>du = e^x \,dx</m>, so <m>dx = \frac{du}{e^x} = \frac{du}{u}</m>. </p>
            <p>
              The integral becomes:
            </p>
            <me>
              \int \frac{1}{u^2-u-2} \cdot \frac{du}{u} = \int \frac{du}{u(u^2-u-2)}
            </me>
            <p> Factor the denominator: <m>u(u^2-u-2) = u(u-2)(u+1)</m>. </p>
            <p>
              Now use partial fractions:
            </p>
            <me>
              \frac{1}{u(u-2)(u+1)} = \frac{A}{u} + \frac{B}{u-2} + \frac{C}{u+1}
            </me>
            <p> Multiply by the denominator: <me>
                1 = A(u-2)(u+1) + Bu(u+1) + Cu(u-2)
              </me> To solve for <m>
              A</m>, let <m>u=0</m>: <m>1 = A(-2)(1) \implies A = -\frac{1}{2}</m>. To solve for <m>
              B</m>, let <m>u=2</m>: <m>1 = B(2)(3) \implies B = \frac{1}{6}</m>. To solve for <m>C</m>,
              let <m>u=-1</m>: <m>1 = C(-1)(-3) \implies C = \frac{1}{3}</m>. </p>
            <p> The decomposition is <me>\frac{-1/2}{u} + \frac{1/6}{u-2} + \frac{1}{3(u+1)}</me>. </p>
            <p>
              Now we integrate:
            </p>
            <me>
              \int \left( -\frac{1}{2u} + \frac{1}{6(u-2)} + \frac{1}{3(u+1)} \right) \,du
            </me>
            <me>
              = -\frac{1}{2}\ln|u| + \frac{1}{6}\ln|u-2| + \frac{1}{3}\ln|u+1| + C
            </me>
            <p> Finally, substitute back <m>u = e^x</m>: </p>
            <me>
              = -\frac{1}{2}\ln(e^x) + \frac{1}{6}\ln|e^x-2| + \frac{1}{3}\ln|e^x+1| + C
            </me>
            <me>
              = -\frac{1}{2}x + \frac{1}{6}\ln|e^x-2| + \frac{1}{3}\ln(e^x+1) + C
            </me>
          </solution>
        </exercise>
      </exercises>
    </section>
  </article>
</pretext>
