<?xml version="1.0" encoding="UTF-8"?>

<pretext xmlns:xi="http://www.w3.org/2001/XInclude">
  <article>
    <section xml:id="ps06-section">
      <title>Problem Set 6</title>

      <subtitle>Volume by Cylindrical Shells and Arc Length</subtitle>
      <xi:include href="ps01.ptx" xpointer="xpointer(//section[1]/introduction)" />
      <exercises>
        <exercise xml:id="ex-shells-method">
          <statement>
            <p> Find the volume of the solid generated by rotating the region bounded by <m>y=x^2</m>
              , <m>x=1</m>, and the <m>x</m>-axis about the <m>y</m>-axis. </p>
          </statement>

          <solution>
            <p> Since we are rotating about the <m>y</m>-axis, the method of cylindrical shells is a
              good choice. The formula is: <me>
                V = \int_a^b 2\pi x f(x) \,dx
              </me> The region is
              bounded by <m>y=x^2</m>, <m>x=1</m>, and <m>y=0</m> (the x-axis). The limits of
              integration are from <m>x=0</m> to <m>x=1</m>. The height of a cylindrical shell at a
              given <m>x</m> is <m>f(x)=x^2</m>. </p>
            <md>
              <mrow>V \amp = \int_0^1 2\pi x (x^2) \,dx</mrow>
              <mrow>\amp = 2\pi \int_0^1 x^3 \,dx</mrow>
              <mrow>\amp = 2\pi \left[ \frac{x^4}{4} \right]_0^1</mrow>
              <mrow>\amp = 2\pi \left( \frac{1^4}{4} - \frac{0^4}{4} \right) = \frac{2\pi}{4} =
                \frac{\pi}{2}</mrow>
            </md>
          </solution>
        </exercise>

        <exercise xml:id="ex-arc-length-revised">
          <statement>
            <p> Find the exact length of the curve given by <m>y = \frac{x^3}{6} + \frac{1}{2x}</m>
              for <m>1 \le x \le 2</m>. </p>
          </statement>

          <solution>
            <p> The formula for arc length is <me>
                L = \int_a^b \sqrt{1 + \left( \frac{dy}{dx} \right)^2} \,dx
              </me>.
              First, we find the derivative: <me>
                \frac{dy}{dx} = \frac{3x^2}{6} - \frac{1}{2x^2} = \frac{x^2}{2} - \frac{1}{2x^2}
              </me>
              Next, we find the term under the square root: <md>
                <mrow>\left( \frac{dy}{dx} \right)^2 \amp = \left( \frac{x^2}{2} - \frac{1}{2x^2}
              \right)^2 = \frac{x^4}{4} - 2\left(\frac{x^2}{2}\right)\left(\frac{1}{2x^2}\right) +
              \frac{1}{4x^4}</mrow>
                <mrow>\amp = \frac{x^4}{4} - \frac{1}{2} + \frac{1}{4x^4}</mrow>
              </md>
              Now, add 1 to this expression: <md>
                <mrow>1 + \left( \frac{dy}{dx} \right)^2 \amp = 1 + \frac{x^4}{4} - \frac{1}{2} +
              \frac{1}{4x^4}</mrow>
                <mrow>\amp = \frac{x^4}{4} + \frac{1}{2} + \frac{1}{4x^4} = \left( \frac{x^2}{2} +
              \frac{1}{2x^2} \right)^2</mrow>
              </md> The term under the square root
              simplifies nicely. </p>

            <p> Now, we set up and evaluate the integral for the arc length: <md>
                <mrow>L \amp = \int_1^2 \sqrt{\left( \frac{x^2}{2} + \frac{1}{2x^2} \right)^2} \,dx</mrow>
                <mrow>\amp = \int_1^2 \left( \frac{x^2}{2} + \frac{1}{2x^2} \right) \,dx</mrow>
                <mrow>\amp = \left[ \frac{x^3}{6} - \frac{1}{2x} \right]_1^2</mrow>
                <mrow>\amp = \left( \frac{2^3}{6} - \frac{1}{2(2)} \right) - \left( \frac{1^3}{6} -
              \frac{1}{2(1)} \right)</mrow>
                <mrow>\amp = \left( \frac{8}{6} - \frac{1}{4} \right) - \left( \frac{1}{6} -
              \frac{1}{2} \right)</mrow>
                <mrow>\amp = \left( \frac{4}{3} - \frac{1}{4} \right) - \left( \frac{1}{6} -
              \frac{3}{6} \right) = \frac{13}{12} - \left(-\frac{2}{6}\right) = \frac{13}{12} +
              \frac{1}{3} = \frac{17}{12}</mrow>
              </md>
            </p>
          </solution>
        </exercise>

        <exercise xml:id="ex-shells-method-2">
          <statement>
            <p> Find the volume of the solid generated by rotating the region bounded by <m>y=x-x^2</m>
              and the <m>x</m>-axis about the line <m>x=2</m>. </p>
          </statement>

          <solution>
            <p> The region is bounded by <m>y=x-x^2</m> and <m>y=0</m>. We find the intersection
              points by setting <m>x-x^2=0</m>, which gives <m>x(1-x)=0</m>, so the intersections
              are at <m>x=0</m> and <m>x=1</m>. When using the shell method, the radius of a shell
              is the distance from the axis of rotation (<m>x=2</m>) to the shell's position at <m>x</m>.
              This distance is <m>r(x)=2-x</m>. The height of a shell at <m>x</m> is the function
              itself, <m>h(x) = y = x-x^2</m>. The limits of integration are from 0 to 1. The volume
              is given by the integral: <me>
                V = \int_a^b 2\pi r(x) h(x) \,dx
              </me>
            </p>
            <md>
              <mrow>V \amp = \int_0^1 2\pi(2-x)(x-x^2) \,dx</mrow>
              <mrow>\amp = 2\pi \int_0^1 (2x-2x^2-x^2+x^3) \,dx</mrow>
              <mrow>\amp = 2\pi \int_0^1 (x^3 - 3x^2 + 2x) \,dx</mrow>
              <mrow>\amp = 2\pi \left[ \frac{x^4}{4} - x^3 + x^2 \right]_0^1</mrow>
              <mrow>\amp = 2\pi \left[ \left(\frac{1^4}{4} - 1^3 + 1^2\right) - \left(0 - 0 +
                0\right) \right]</mrow>
              <mrow>\amp = 2\pi \left[ \frac{1}{4} - 1 + 1 \right] = 2\pi \left( \frac{1}{4} \right)
                = \frac{\pi}{2}</mrow>
            </md>
          </solution>
        </exercise>

        <exercise xml:id="ex-arc-length-2">
          <statement>
            <p> Find the length of the curve defined by <m>y = \ln(\cos x)</m> from <m>x=0</m> to <m>
              x=\frac{\pi}{4}</m>. </p>
          </statement>

          <solution>
            <p> The arc length formula is <me>
                L = \int_a^b \sqrt{1 + (y')^2} \,dx
              </me>. First, we
              find the derivative <m>y'</m>: <me>
                y' = \frac{d}{dx}(\ln(\cos x)) = \frac{1}{\cos x} (-\sin x) = -\tan x
              </me>
              Next, we find the term under the square root: <me>
                1 + (y')^2 = 1 + (-\tan x)^2 = 1+\tan^2 x = \sec^2 x
              </me>
              The integral becomes: <me>
                L = \int_0^{\pi/4} \sqrt{\sec^2 x} \,dx = \int_0^{\pi/4} |\sec x| \,dx
              </me>
              Since <m>\sec x &gt; 0</m> on the interval <m>[0, \pi/4]</m>, we can remove the
              absolute value. <me>
                L = \int_0^{\pi/4} \sec x \,dx = \left[ \ln|\sec x + \tan x| \right]_0^{\pi/4}
              </me>
              Now we evaluate the definite integral: </p>
            <md>
              <mrow>L \amp = \left( \ln|\sec(\pi/4) + \tan(\pi/4)| \right) - \left( \ln|\sec(0) +
                \tan(0)| \right)</mrow>
              <mrow>\amp = \left( \ln|\sqrt{2} + 1| \right) - \left( \ln|1 + 0| \right)</mrow>
              <mrow>\amp = \ln(\sqrt{2} + 1) - \ln(1) = \ln(\sqrt{2} + 1)</mrow>
            </md>
          </solution>
        </exercise>
      </exercises>
    </section>
  </article>
</pretext>